added a `at` clause for `ite_cases`

util/meta/tactic/ite.lean
@@ -1,40 +1,59 @@
 
+namespace interactive
+
+open tactic
+
+meta def loc.get_locations : loc → tactic (list expr)
+| loc.wildcard := (::) <$> tactic.target <*> (tactic.local_context >>= mmap infer_type)
+| (loc.ns xs)  := mmap (λ n, match n with
+  | none :=   tactic.target
+  | some n := tactic.get_local n >>= infer_type
+  end) xs
+
+end interactive
+
 namespace tactic.interactive
 
 open lean lean.parser  interactive
 open interactive.types
 open tactic
 
+local postfix `?`:9001 := optional
+local postfix *:9001 := many
+
 meta def find_ite : expr → ℕ →
-  option (bool × expr × expr × expr × expr) →
-  option (bool × expr × expr × expr × expr)
+  option (bool × expr × expr) →
+  option (bool × expr × expr)
 | `(@ite %%c %%d %%α %%l %%r) i none :=
-  if ¬ c.has_var then some (ff, c, d, l, r)
+  if ¬ c.has_var then some (ff, c, d)
                  else none
 | `(@dite %%c %%d %%α %%l %%r) i none :=
-  if ¬ c.has_var then some (tt, c, d, l, r)
+  if ¬ c.has_var then some (tt, c, d)
                  else none
 | e i none := none
 | _ _ (some e) := (some e)
 
-meta def ite_cases (hyp : parse (tk "with" *> ident)) : tactic unit :=
-do g ← target,
-   match expr.fold g none find_ite with
-    | (some (_,e,d,l,r)) :=
-      do cases (none,to_pexpr d) [hyp,hyp]
-         ; [ (do hyp ← get_local hyp,
+meta def ite_cases (hyp : parse (tk "with" *> ident_) ?)
+                   (ls : parse location)
+: tactic unit :=
+do g ← ls.get_locations >>= mmap instantiate_mvars,
+   match list.foldl (λ r e, expr.fold e r find_ite) none g with
+    | (some (_,e,d)) :=
+      do hyp' ← get_unused_name $ option.cases_on hyp `h id,
+         cases (none,to_pexpr d) [hyp',hyp']
+         ; [ (do hyp' ← get_local hyp',
                  simp tt [ simp_arg_type.expr
-                            ``(@dif_neg _ (is_false %%hyp) %%hyp)
+                            ``(@dif_neg _ (is_false %%hyp') %%hyp')
                          , simp_arg_type.expr
-                            ``(@if_neg _ (is_false %%hyp) %%hyp)]
-                         [] (loc.ns [none]))
-           , do hyp ← get_local hyp,
+                            ``(@if_neg _ (is_false %%hyp') %%hyp')]
+                         [] ls)
+           , do hyp' ← get_local hyp',
                 simp tt [ simp_arg_type.expr
-                           ``(@dif_pos _ (is_true %%hyp) %%hyp)
+                           ``(@dif_pos _ (is_true %%hyp') %%hyp')
                         , simp_arg_type.expr
-                           ``(@if_pos _ (is_true %%hyp) %%hyp)]
-                        [] (loc.ns [none]) ]
-    | none :=  fail "no conidition found"
+                           ``(@if_pos _ (is_true %%hyp') %%hyp')]
+                        [] ls ]
+    | none :=  fail "no conditionals found"
    end
 
 example (x y : ℕ)
@@ -71,6 +90,29 @@ example (x y i j : ℕ)
 begin
   ite_cases with h₃,
   all_goals { assumption }
+end
+
+example (x y i j : ℕ)
+  (f : ℕ → ℕ)
+  (h'' : (if h : x ≤ y then x ≤ i else y ≤ j))
+  (h''' : f (if h : x ≤ y then y else x) ≤ 7)
+  (h'''' : (if h : x ≤ y then y else x) ≤ 7)
+: (if h : x ≤ y then x else y) ≤ (if x ≤ y then i else j) :=
+begin
+  ite_cases with h₃ at ⊢ h'' h''',
+  all_goals { assumption }
+end
+
+example (x y i j : ℕ)
+  (f : ℕ → ℕ)
+  (h'' : (if h : x ≤ y then x ≤ i else y ≤ j))
+  (h''' : f (if h : x ≤ y then y else x) ≤ 7)
+  (h'''' : (if h : x ≤ y then y else x) ≤ 7)
+: x ≤ i ∨ y ≤ j :=
+begin
+  ite_cases with h₃ at ⊢ h'' h'''
+  ; [ right , left ]
+  ; assumption
 end
 
 end tactic.interactive
